fix word_inst for load/store byte and prove everyhting in word_to_stack except comp_Call_correct

compiler/backend/semantics/wordPropsScript.sml
@@ -3335,6 +3335,13 @@ val full_inst_ok_less_def = Define`
       (case handler of
         NONE => T
       | SOME (n,h,l1,l2) => full_inst_ok_less c h))) ∧
+  (full_inst_ok_less c (ShareInst op r ad) =
+    case exp_to_addr ad of
+    | SOME (Addr _ w) =>
+      if op IN {Load; Store}
+        then addr_offset_ok c w 
+        else byte_offset_ok c w
+    | NONE => F) ∧
   (full_inst_ok_less c prog ⇔ T)`
 
 (* All cutsets are well-formed *)
